lib/steel/pulse/Pulse.Soundness.Exists.fsti
@@ -8,14 +8,14 @@ open Pulse.Soundness.Common
 
 module RT = FStar.Reflection.Typing
 
-val intro_exists_erased_soundness
-  (#g:stt_env)
-  (#t:st_term)
-  (#c:comp)
-  (d:st_typing g t c{T_IntroExistsErased? d})
-  : GTot (RT.tot_typing (elab_env g)
-                        (elab_st_typing d)
-                        (elab_comp c))
+// val intro_exists_erased_soundness
+//   (#g:stt_env)
+//   (#t:st_term)
+//   (#c:comp)
+//   (d:st_typing g t c{T_IntroExistsErased? d})
+//   : GTot (RT.tot_typing (elab_env g)
+//                         (elab_st_typing d)
+//                         (elab_comp c))
 
 val intro_exists_soundness
   (#g:stt_env)
@@ -34,5 +34,3 @@ val elim_exists_soundness
   : GTot (RT.tot_typing (elab_env g)
                         (elab_st_typing d)
                         (elab_comp c))
-
-
