lib/steel/pulse/Pulse.Syntax.Printer.fst
@@ -197,19 +197,19 @@ let rec st_term_to_string' (level:string) (t:st_term)
       sprintf "elim_exists %s"
         (term_to_string p)
 
-    | Tm_IntroExists { erased=false; p; witnesses } ->
+    | Tm_IntroExists { p; witnesses } ->
       sprintf "introduce\n%s%s\n%swith %s"
         (indent level)
         (term_to_string' (indent level) p)
         level
         (term_list_to_string " " witnesses)
 
-    | Tm_IntroExists { erased=true; p; witnesses } ->
-      sprintf "introduce (erased)\n%s%s\n%swith %s"
-        (indent level)
-        (term_to_string' (indent level) p)
-        level
-        (term_list_to_string " " witnesses)
+    // | Tm_IntroExists { erased=true; p; witnesses } ->
+    //   sprintf "introduce (erased)\n%s%s\n%swith %s"
+    //     (indent level)
+    //     (term_to_string' (indent level) p)
+    //     level
+    //     (term_list_to_string " " witnesses)
 
     | Tm_While { invariant; condition; body } ->
       sprintf "while (%s)\n%sinvariant %s\n%s{\n%s%s\n%s}"
